Examples/TicketLock.v
@@ -16,13 +16,16 @@ From LHL.Examples Require Import
   VarSpec.
 
 From LHL.Util Require Import
-  Tactics.
+  Tactics
+  TransUtil
+  Util.
 
 From Coq Require Import
   Arith.PeanoNat
   Program.Equality
   Logic.FunctionalExtensionality
-  Logic.PropExtensionality.
+  Logic.PropExtensionality
+  Logic.Classical_Prop.
 
 Definition Underlay := FAISig |+| CounterSig |+| VarSig nat.
 
@@ -69,6 +72,113 @@ Definition mytkt i (s : @InterState E F VE) : option nat :=
   | VarSet n _ => Some n
   end.
 
+Definition Inv (i : ThreadName) : Prec :=
+  fun s ρs => exists ρ, ρs = eq ρ /\
+    countState s <> CounterUB /\
+    (forall tkt,
+      Some tkt = mytkt i s ->
+      ctrval s <= tkt) /\
+    ctrval s <= newtkt s /\
+    (mytkt i s = Some (ctrval s) ->
+      owner (PState ρ) = Some i \/ owner (PState ρ) = None) /\
+    (newtkt s = ctrval s ->
+      PState ρ = LockUnowned) /\
+    (owner (PState ρ) = Some i ->
+      mytkt i s = Some (ctrval s)).
+
+Definition Acqed (i : ThreadName) : Prec := fun s ρs =>
+  exists ρ, ρs = eq ρ /\
+  (owner (PState ρ) = Some i /\ Inv i s ρs) \/
+  (owner (PState ρ) <> Some i).
+
+Definition Reled (i : ThreadName) : Prec := fun s ρs =>
+  exists ρ, ρs = eq ρ /\
+  (owner (PState ρ) <> Some i /\ Inv i s ρs) \/
+  (owner (PState ρ) = Some i).
+
+Definition Precs (i : ThreadName) {A} (m : LockSig A) : Prec :=
+  fun s ρs => exists ρ, ρs = eq ρ /\
+    match m with
+    | Acq =>
+        owner (PState ρ) <> Some i ->
+          Inv i s ρs
+    | Rel =>
+        owner (PState ρ) = Some i ->
+          Inv i s ρs
+    end.
+
+Definition Posts (i : ThreadName) {A} (m : LockSig A) : Post A :=
+  fun _ s ρs t σs => forall ρ, ρs = eq ρ -> exists σ, σs = eq σ /\
+    match m with
+    | Acq =>
+        owner (PState ρ) <> Some i ->
+          owner (PState σ) = Some i /\
+          Inv i t σs
+    | Rel =>
+        owner (PState ρ) = Some i ->
+          owner (PState σ) <> Some i /\
+          Inv i t σs
+    end.
+
+Definition ManyInvokeReturn i : Relt :=
+  RTC (fun s ρs t σs =>
+    exists j, j <> i /\
+      (InvokeAny ticketLockImpl j s ρs t σs \/
+       ReturnAny ticketLockImpl j s ρs t σs)).
+
+Definition Rely (i : ThreadName) : Relt :=
+  fun s ρs t σs => forall ρ, ρs = eq ρ -> exists σ, σs = eq σ /\ (
+    ManyInvokeReturn i s ρs t σs \/
+    (countState s <> CounterUB ->
+      countState t <> CounterUB) /\
+    ((forall tkt, Some tkt = mytkt i s -> ctrval s <= tkt) ->
+      forall tkt',
+      Some tkt' = mytkt i t ->
+      ctrval t <= tkt') /\
+    (ctrval s <= newtkt s ->
+      ctrval t <= newtkt t) /\
+    ((mytkt i s = Some (ctrval s) -> owner (PState ρ) = Some i \/ owner (PState ρ) = None) ->
+      mytkt i t = Some (ctrval t) ->
+      owner (PState σ) = Some i \/ owner (PState σ) = None) /\
+    ((newtkt s = ctrval s -> PState ρ = LockUnowned) ->
+      newtkt t = ctrval t ->
+      PState σ = LockUnowned) /\
+    ((owner (PState ρ) = Some i -> mytkt i s = Some (ctrval s)) ->
+      owner (PState σ) = Some i ->
+      mytkt i t = Some (ctrval t)) /\
+    (owner (PState ρ) = Some i <-> owner (PState σ) = Some i) /\
+    (owner (PState ρ) = Some i ->
+      PState ρ = PState σ /\
+      countState s = countState t) /\
+    (owner (PState ρ) <> Some i <-> owner (PState σ) <> Some i) /\
+    fst s i = fst t i
+  ).
+
+Definition Guar (i : ThreadName) : Relt :=
+  fun s ρs t σs =>
+    forall j, i <> j -> Rely j s ρs t σs.
+
+(* Extra lemmas *)
+
+Lemma tollens {P Q : Prop} :
+  ~Q -> (P -> Q) -> ~P.
+tauto.
+Qed.
+
+Lemma eq_inj {A} :
+  forall x y : A, eq x = eq y -> x = y.
+intros.
+assert (forall z, eq x z = eq z y).
+{
+  intros. apply propositional_extensionality.
+  split; intros.
+  rewrite H in H0. easy.
+  rewrite H. easy.
+}
+specialize (H0 x).
+rewrite <- H0. easy.
+Qed.
+
 Lemma newtkt_eq :
   forall s t : @InterState E F VE,
   snd s = snd t ->
@@ -100,86 +210,18 @@ unfold countState. intros.
 rewrite H. easy.
 Qed.
 
-Definition Inv (i : ThreadName) : Prec :=
-  fun s ρs => exists ρ, ρs = eq ρ /\
-    countState s <> CounterUB /\
-    (forall tkt,
-      Some tkt = mytkt i s ->
-      ctrval s <= tkt) /\
-    ctrval s <= newtkt s /\
-    (mytkt i s = Some (ctrval s) ->
-      owner (PState ρ) = Some i \/ owner (PState ρ) = None) /\
-    (newtkt s = ctrval s ->
-      PState ρ = LockUnowned) /\
-    (owner (PState ρ) = Some i ->
-      mytkt i s = Some (ctrval s)).
-
-Definition Acqed (i : ThreadName) : Prec := fun s ρs =>
-  exists ρ, ρs = eq ρ /\
-  (owner (PState ρ) = Some i ->
-    Inv i s ρs).
-
-Definition Reled (i : ThreadName) : Prec := fun s ρs =>
-  exists ρ, ρs = eq ρ /\
-  (owner (PState ρ) <> Some i ->
-    Inv i s ρs).
-
-Definition Precs (i : ThreadName) {A} (m : LockSig A) : Prec :=
-  fun s ρs =>
-    match m with
-    | Acq => Reled i s ρs
-    | Rel => Acqed i s ρs
-    end.
-
-Definition Posts (i : ThreadName) {A} (m : LockSig A) : Post A :=
-  fun _ _ _ t σ =>
-    match m with
-    | Acq => Acqed i t σ
-    | Rel => Reled i t σ
-    end.
-
-Definition ManyInvokeReturn i : Relt :=
-  RTC (fun s ρs t σs =>
-    exists j, j <> i /\
-      (InvokeAny ticketLockImpl j s ρs t σs \/
-       ReturnAny ticketLockImpl j s ρs t σs)).
-
-Definition Rely (i : ThreadName) : Relt :=
-  fun s ρs t σs => forall ρ, ρs = eq ρ -> exists σ, σs = eq σ /\ (
-    ManyInvokeReturn i s ρs t σs \/
-    (countState s <> CounterUB ->
-      countState t <> CounterUB) /\
-    ((forall tkt, Some tkt = mytkt i s -> ctrval s <= tkt) ->
-      forall tkt',
-      Some tkt' = mytkt i t ->
-      ctrval t <= tkt') /\
-    (ctrval s <= newtkt s ->
-      ctrval t <= newtkt t) /\
-    ((mytkt i s = Some (ctrval s) -> owner (PState ρ) = Some i \/ owner (PState ρ) = None) ->
-      mytkt i t = Some (ctrval t) ->
-      owner (PState σ) = Some i \/ owner (PState σ) = None) /\
-    ((newtkt s = ctrval s -> PState ρ = LockUnowned) ->
-      newtkt t = ctrval t ->
-      PState σ = LockUnowned) /\
-    ((owner (PState ρ) = Some i -> mytkt i s = Some (ctrval s)) ->
-      owner (PState σ) = Some i ->
-      mytkt i t = Some (ctrval t)) /\
-    (owner (PState ρ) = Some i ->
-      PState ρ = PState σ /\
-      ctrval s = ctrval t) /\
-    (owner (PState ρ) <> Some i ->
-      owner (PState σ) <> Some i)
-  ).
-
-Definition Guar (i : ThreadName) : Relt :=
-  fun s ρs t σs =>
-    forall j, i <> j -> Rely j s ρs t σs.
-
-(* Extra lemmas *)
+Lemma cntSt_to_ctrval :
+  forall s t : @InterState E F VE,
+  countState s = countState t ->
+  ctrval s = ctrval t.
+unfold ctrval. intros.
+rewrite H. easy.
+Qed.
 
 Lemma noStateChange :
   forall i s ρs t σs,
   ManyInvokeReturn i s ρs t σs ->
+  fst s i = fst t i /\
   snd s = snd t /\
   forall σ, σs σ ->
     exists ρ, ρs ρ /\
@@ -188,29 +230,32 @@ intros.
 induction H.
 {
   split. easy.
+  split. easy.
   intros. exists σ. easy.
 }
 {
   clear H0.
   destruct_all.
-  destruct H2.
+  destruct H3.
   {
-    unfold InvokeAny, TInvoke in H2. destruct_all.
-    destruct H3. simpl in *.
+    unfold InvokeAny, TInvoke, mapInvPoss in H3. psimpl.
+    destruct H4. cbn in *.
+    split. transitivity (fst t i). apply H7. easy. easy.
     split. transitivity (snd t); easy.
-    intros.
-    apply H1 in H7. destruct_all.
-    apply H5 in H7. destruct_all.
+    intros. apply H2 in H8. clear H2. psimpl.
+    destruct H6. clear H6.
+    apply H9 in H2. psimpl.
     exists x3. split. easy.
     congruence.
   }
   {
-    unfold ReturnAny, TReturn in H2. destruct_all.
-    destruct H2. simpl in *.
+    unfold ReturnAny, TReturn, mapRetPoss in H3. psimpl.
+    destruct H3. cbn in *.
+    split. transitivity (fst t i). apply H6. easy. easy.
     split. transitivity (snd t); easy.
-    intros.
-    apply H1 in H6. destruct_all.
-    apply H4 in H6. destruct_all.
+    intros. apply H2 in H7. clear H2. psimpl.
+    destruct H5. clear H5.
+    apply H8 in H2. psimpl.
     exists x4. split. easy.
     congruence.
   }
@@ -226,17 +271,133 @@ exists x0. split. easy.
 destruct H0.
 {
   apply noStateChange in H. destruct_all.
-  specialize (H0 x0 eq_refl). destruct_all. subst.
-  rewrite <- H7. symmetry in H.
-  repeat rewrite (countState_eq _ _ H).
-  repeat rewrite (newtkt_eq _ _ H).
-  repeat rewrite (mytkt_eq _ _ _ H).
-  repeat rewrite (ctrval_eq _ _ H).
+  specialize (H7 x0 eq_refl). destruct_all. subst.
+  rewrite <- H8. symmetry in H0.
+  repeat rewrite (countState_eq _ _ H0).
+  repeat rewrite (newtkt_eq _ _ H0).
+  repeat rewrite (mytkt_eq _ _ _ H0).
+  repeat rewrite (ctrval_eq _ _ H0).
   easy.
 }
 {
   destruct_all.
   repeat split; auto.
+}
+Qed.
+
+Lemma Rely_pres_single :
+  forall i s ρ t σs,
+  Rely i s (eq ρ) t σs ->
+  exists σ, σs = eq σ.
+unfold Rely. intros.
+specialize (H ρ eq_refl). psimpl.
+exists x. easy.
+Qed.
+
+Lemma Rely_pres_not_owned :
+  forall i s ρ t σ,
+  Rely i s (eq ρ) t (eq σ) ->
+  owner (PState σ) <> Some i <->
+  owner (PState ρ) <> Some i.
+unfold Rely. intros. specialize (H ρ eq_refl). psimpl.
+apply eq_inj in H. subst.
+destruct H0.
+{
+  apply noStateChange in H. psimpl.
+  specialize (H1 x eq_refl). psimpl.
+  rewrite H2. easy.
+}
+{
+  psimpl. easy.
+}
+Qed.
+
+
+Lemma Rely_pres_owned :
+  forall i s ρ t σ,
+  Rely i s (eq ρ) t (eq σ) ->
+  owner (PState σ) = Some i <->
+  owner (PState ρ) = Some i.
+unfold Rely. intros. specialize (H ρ eq_refl). psimpl.
+apply eq_inj in H. subst.
+destruct H0.
+{
+  apply noStateChange in H. psimpl.
+  specialize (H1 x eq_refl). psimpl.
+  rewrite H2. easy.
+}
+{
+  psimpl. easy.
+}
+Qed.
+
+Lemma mapPossInv_pres_single :
+  forall i ρ σs A (m : F A),
+  mapPoss (VF:=VF) (eq ρ) σs (mapInvPoss i m) ->
+  exists σ, σs = eq σ.
+unfold mapInvPoss. intros.
+destruct H. specialize (H ρ eq_refl). destruct_all.
+exists x. extensionality x1. apply propositional_extensionality.
+split; intros.
+{
+  apply H0 in H8. clear H0. destruct_all. subst.
+  destruct x, x0, x1. cbn in *.
+  f_equal.
+  { congruence. }
+  {
+    extensionality k.
+    dec_eq_nats i k.
+    congruence.
+    etransitivity.
+    apply H5. easy.
+    symmetry. apply H12. easy.
+  }
+  {
+    extensionality k.
+    dec_eq_nats i k.
+    congruence.
+    etransitivity.
+    apply H6. easy.
+    symmetry. apply H13. easy.
+  }
+}
+{
+  subst. easy.
+}
+Qed.
+
+Lemma mapPossRet_pres_single :
+  forall i ρ σs A (m : F A) v,
+  mapPoss (VF:=VF) (eq ρ) σs (mapRetPoss i m v) ->
+  σs = eq (retPoss i ρ).
+unfold mapRetPoss. intros. destruct H.
+specialize (H ρ eq_refl). destruct_all.
+extensionality x0. apply propositional_extensionality.
+split; intros.
+{
+  apply H0 in H8. clear H0. psimpl.
+  unfold retPoss. destruct x1, x0. psimpl.
+  f_equal.
+  extensionality j. dec_eq_nats i j.
+  rewrite eqb_id. easy.
+  rewrite eqb_nid. symmetry. apply H12; easy. easy.
+  extensionality j. dec_eq_nats i j.
+  rewrite eqb_id. easy.
+  rewrite eqb_nid. symmetry. apply H13; easy. easy.
+}
+{
+  subst. assert (H' := H).
+  apply H0 in H'. clear H0. psimpl.
+  assert (x = retPoss i x0).
+  destruct x, x0. unfold retPoss. psimpl.
+  f_equal.
+  extensionality j. dec_eq_nats i j.
+  rewrite eqb_id. easy.
+  rewrite eqb_nid. apply H5. easy. easy.
+  extensionality j. dec_eq_nats i j.
+  rewrite eqb_id. easy.
+  rewrite eqb_nid. apply H6. easy. easy.
+  subst. easy.
 }
 Qed.
 
@@ -264,39 +425,47 @@ destruct H0, H1.
 {
   right.
   apply noStateChange in H. destruct_all.
-  move H at bottom. symmetry in H.
-  specialize (H8 x0 eq_refl). destruct_all. subst.
-  symmetry in H9. move H9 at bottom.
-  repeat rewrite (countState_eq _ _ H).
-  repeat rewrite (ctrval_eq _ _ H).
-  repeat rewrite (mytkt_eq _ _ _ H).
-  repeat rewrite (newtkt_eq _ _ H).
-  repeat rewrite H9.
+  move H10 at bottom. symmetry in H10.
+  specialize (H11 x0 eq_refl). destruct_all. subst.
+  symmetry in H12. move H12 at bottom.
+  repeat rewrite (countState_eq _ _ H10) in *.
+  repeat rewrite (ctrval_eq _ _ H10) in *.
+  repeat rewrite (mytkt_eq _ _ _ H10) in *.
+  repeat rewrite (newtkt_eq _ _ H10) in *.
+  repeat rewrite H12 in *.
+  rewrite H9.
   easy.
 }
 {
   right.
   apply noStateChange in H0. destruct_all.
-  specialize (H1 x1 eq_refl). destruct_all. subst.
-  symmetry in H9. move H9 at bottom.
-  repeat rewrite (countState_eq _ _ H0) in *.
-  repeat rewrite (ctrval_eq _ _ H0) in *.
-  repeat rewrite (mytkt_eq _ _ _ H0) in *.
-  repeat rewrite (newtkt_eq _ _ H0) in *.
-  repeat rewrite H9 in *.
+  specialize (H2 x1 eq_refl). destruct_all. subst.
+  symmetry in H1. move H1 at bottom.
+  repeat rewrite (countState_eq _ _ H1) in *.
+  repeat rewrite (ctrval_eq _ _ H1) in *.
+  repeat rewrite (mytkt_eq _ _ _ H1) in *.
+  repeat rewrite (newtkt_eq _ _ H1) in *.
+  repeat rewrite H12 in *.
+  rewrite H0.
   easy.
 }
 {
   right. destruct_all.
-  repeat split; intros; try auto.
-  assert (H15' := H15).
-  apply H6 in H15. destruct_all. rewrite H15 in H15'.
-  apply H13 in H15'. destruct_all.
-  rewrite H15. easy.
-  assert (H15' := H15).
-  apply H6 in H15. destruct_all. rewrite H15 in H15'.
-  apply H13 in H15'. destruct_all.
-  rewrite H16. easy.
+  split. auto.
+  split. auto.
+  split. auto.
+  split. auto.
+  split. auto.
+  split. auto.
+  split. rewrite H6. easy.
+  split.
+  {
+    intros. assert (H19' := H19). apply H7 in H19. psimpl.
+    rewrite H19 in H19'. apply H16 in H19'. psimpl.
+    rewrite H19, H20. easy.
+  }
+  split. rewrite H8. easy.
+  rewrite H9. easy.
 }
 Qed.
 
@@ -312,54 +481,158 @@ unfold InvokeAny, TInvoke, Rely, sub, subRelt, TIdle. intros.
 destruct_all. subst. destruct H2. cbn in *.
 specialize (H5 ρ0 eq_refl). destruct_all.
 assert (exists τ, σ = eq τ).
-{
-  destruct H4. specialize (H4 ρ0 eq_refl). destruct_all.
-  exists x1.
-  extensionality x2. apply propositional_extensionality.
-  split; intros.
-  {
-    apply H7 in H15. clear H7. destruct_all. subst.
-    destruct x1, x2, x3. cbn in *.
-    f_equal.
-    { congruence. }
-    {
-      extensionality k.
-      dec_eq_nats i k.
-      congruence.
-      etransitivity.
-      apply H12. easy.
-      symmetry. apply H19. easy.
-    }
-    {
-      extensionality k.
-      dec_eq_nats i k.
-      congruence.
-      etransitivity.
-      apply H13. easy.
-      symmetry. apply H20. easy.
-    }
-  }
-  {
-    subst. easy.
-  }
-}
+eapply mapPossInv_pres_single. exact H4.
 destruct_all. subst.
 exists x1. split. easy.
 destruct H4. clear H7.
-specialize (H4 ρ0 eq_refl). destruct_all. subst.
+specialize (H4 ρ0 eq_refl).
+unfold mapInvPoss in H4. destruct_all. subst.
 symmetry in H13. repeat rewrite H13.
 repeat rewrite (mytkt_eq _ _ _ H3).
 repeat rewrite (countState_eq _ _ H3).
 repeat rewrite (newtkt_eq _ _ H3).
 repeat rewrite (ctrval_eq _ _ H3).
+rewrite H2. 2: easy.
 right. easy.
 Qed.
 
 Lemma Ret_in_Rely :
   forall i j : ThreadName, i <> j -> ReturnAny ticketLockImpl i ==> Rely j.
 unfold ReturnAny, TReturn, Rely, sub, subRelt, TIdle. intros.
-destruct_all. subst. destruct H3. cbn in *.
-Admitted.
+destruct_all. subst. cbn in *.
+assert (σ = eq (retPoss i ρ0)).
+eapply mapPossRet_pres_single. exact H3.
+destruct_all. subst. destruct H3.
+exists (retPoss i ρ0). split. easy.
+destruct H0.
+specialize (H1 ρ0 eq_refl). specialize (H3 (retPoss i ρ0) eq_refl).
+psimpl. unfold mapRetPoss in H6. psimpl.
+symmetry in H9. repeat rewrite H9.
+symmetry in H2.
+repeat rewrite (mytkt_eq _ _ _ H2).
+repeat rewrite (countState_eq _ _ H2).
+repeat rewrite (newtkt_eq _ _ H2).
+repeat rewrite (ctrval_eq _ _ H2).
+rewrite H4. 2: easy.
+right. easy.
+Qed.
+
+Lemma init_in_Precs :
+  forall i A (m : LockSig A), Precs i m (allIdle, Init VE) (eq initPoss).
+unfold Precs, Reled, Acqed, Inv. intros.
+exists initPoss. split. easy.
+destruct m; simpl.
+{
+  intros. exists initPoss. split. easy.
+  easy.
+}
+{
+  intros. exists initPoss. split. easy.
+  easy.
+}
+Qed.
+
+Ltac decide_prop P :=
+  let H := fresh in
+  assert (H : P \/ ~P) by apply excluded_middle;
+  destruct H.
+
+Lemma Precs_stable :
+  forall i A (m : LockSig A), Stable (Rely i) (Precs i m).
+unfold Precs, Acqed, Reled. intros. destruct m.
+{
+  unfold Stable, stablePrec, sub, subPrec. intros. psimpl.
+  assert (exists τ, ρ = eq τ).
+  eapply Rely_pres_single. exact H0. psimpl.
+  exists x0. split. easy. intros.
+  assert (owner (PState x1) <> Some i).
+  eapply (Rely_pres_not_owned _ _ _ _ _ H0). easy.
+  apply H1 in H2. clear H1.
+  apply Inv_stable.
+  psplit. exact H2. easy.
+}
+{
+  unfold Stable, stablePrec, sub, subPrec. intros. psimpl.
+  assert (exists τ, ρ = eq τ).
+  eapply Rely_pres_single. exact H0. psimpl.
+  exists x0. split. easy. intros.
+  assert (owner (PState x1) = Some i).
+  eapply (Rely_pres_owned _ _ _ _ _ H0). easy.
+  apply H1 in H2. clear H1.
+  apply Inv_stable.
+  psplit. exact H2. easy.
+}
+Qed.
+
+Lemma Posts_stable :
+  forall i A (m : LockSig A) v, Stable (Rely i) (Posts i m v).
+unfold Posts, Acqed, Reled. intros. destruct m.
+{
+  unfold Stable, stablePost, stableRelt, sub, subRelt.
+  split; intros; psimpl.
+  {
+    assert (exists τ, x0 = eq τ).
+    eapply Rely_pres_single. exact H. psimpl.
+    specialize (H1 x1 eq_refl). psimpl.
+    exists x0. split. easy.
+    intros. apply H1.
+    eapply Rely_pres_not_owned.
+    exact H. easy.
+  }
+  {
+    specialize (H ρ0 eq_refl). psimpl.
+    assert (exists τ, σ = eq τ).
+    eapply Rely_pres_single. exact H1. psimpl.
+    exists x0. split. easy.
+    intros. apply H0 in H. clear H0.
+    psimpl. split.
+    eapply Rely_pres_owned. 
+    exact H1. easy.
+    apply Inv_stable.
+    psplit. exact H0. easy.
+  }
+}
+{
+  unfold Stable, stablePost, stableRelt, sub, subRelt.
+  split; intros; psimpl.
+  {
+    assert (exists τ, x0 = eq τ).
+    eapply Rely_pres_single. exact H. psimpl.
+    specialize (H1 x1 eq_refl). psimpl.
+    exists x0. split. easy.
+    intros. apply H1. clear H1.
+    eapply Rely_pres_owned. exact H.
+    easy. 
+  }
+  {
+    specialize (H ρ0 eq_refl). psimpl.
+    assert (exists τ, σ = eq τ).
+    eapply Rely_pres_single. exact H1. psimpl.
+    exists x0. split. easy.
+    intros. apply H0 in H. clear H0. psimpl.
+    split.
+    eapply Rely_pres_not_owned. exact H1. easy.
+    apply Inv_stable.
+    psplit. exact H0. easy.
+  }
+}
+Qed.
+
+Lemma ticketLockImpl_switch_code :
+  forall i A (m1 : LockSig A) B (m2 : LockSig B) v,
+  prComp (Precs i m1) (Posts i m1 v) <<- PrecToRelt (Returned i m1) <<-
+  TReturn ticketLockImpl i m1 ==>
+  Precs i m2.
+unfold sub, subPrec, Precs, Posts. intros. destruct m1, m2.
+{
+  psimpl. specialize (H2 x5 eq_refl). psimpl.
+  unfold TReturn, InterOStep in H0. psimpl. destruct x0.
+  eapply mapPossRet_pres_single in H4. subst.
+  exists (retPoss i x1). split. easy.
+  simpl. intros.
+  
+}
+Qed.
 
 Theorem ticketLockCorrect :
   VerifyImpl VE VF Rely Guar Precs ticketLockImpl Posts.
@@ -369,3 +642,7 @@ apply Rely_trans.
 apply Guar_in_Rely.
 apply Inv_in_Rely.
 apply Ret_in_Rely.
+apply init_in_Precs.
+apply Precs_stable.
+apply Posts_stable.
+apply ticketLockImpl_switch_code.
